ems/SimModSem.v
@@ -1323,7 +1323,7 @@ Theorem adequacy
   (P Q: Prop)
   ms_src ms_tgt
   (SIM: ModSemPair.sim ms_src ms_tgt)
-  (WF: Q -> P)
+  (WF: P -> Q)
   :
   (Beh.of_program (ModSem.compile ms_tgt (Some P)))
   <1=
@@ -1333,7 +1333,7 @@ Proof.
   inv SIM.
   des. ginit.
   { eapply cpn7_wcompat; eauto with paco. }
-  unfold ModSem.initial_itr, assume.
+  unfold ModSem.initial_itr, guarantee.
   steps.
   force. esplits; et. steps.
   unfold ITree.map. steps. unfold assume. steps. des.
@@ -1361,11 +1361,12 @@ Section SIMMOD.
   Variable (md_src md_tgt: Mod.t).
   Inductive sim: Prop := mk {
     sim_modsem:
-      forall sk
-             (SKINCL: Sk.extends md_tgt.(Mod.sk) sk)
-             (SKWF: Sk.wf sk),
-        <<SIM: ModSemPair.sim (md_src.(Mod.get_modsem) sk) (md_tgt.(Mod.get_modsem) sk)>>;
-    sim_sk: forall (SKWF: Sk.wf md_src.(Mod.sk)), md_src.(Mod.sk) ≡ md_tgt.(Mod.sk);
+      forall sk_src sk_tgt
+             (EXT: Sk.extends sk_src sk_tgt)
+             (SKWF: Sk.wf (sk_tgt ⊕ md_tgt.(Mod.sk))),
+        <<SIM: ModSemPair.sim (md_src.(Mod.get_modsem) (sk_src ⊕ md_src.(Mod.sk)))
+                 (md_tgt.(Mod.get_modsem) (sk_tgt ⊕ md_tgt.(Mod.sk)))>>;
+    sim_sk: Sk.extends md_src.(Mod.sk) md_tgt.(Mod.sk);
   }.
 
 End SIMMOD.
@@ -1386,16 +1387,31 @@ Proof.
   inv SIM1.
   des.
   econs; ss.
-  2:{ i. rewrite sim_sk0.
-      2: { eapply Sk.wf_mon; et. r. esplits; et. refl. }
-      rewrite sim_sk1.
-      2: { eapply Sk.wf_mon; et. r. esplits; et. rewrite Sk.add_comm. refl. }
-      refl.
-  }
+  2:{ i. rewrite sim_sk0. rewrite sim_sk1. refl. }
   ii; ss.
   eapply ModSemPair.compose; et.
-  - eapply sim_modsem0; ss. etrans; et. r. esplits; et. refl.
-  - eapply sim_modsem; ss. etrans; et. r. esplits; et. rewrite Sk.add_comm. refl.
+  - assert(T: sk_src ⊕ (Mod.sk md_src0 ⊕ Mod.sk md_src1) ≡ (sk_src ⊕ Mod.sk md_src1) ⊕ Mod.sk md_src0).
+    { rewrite <- ! Sk.add_assoc. eapply Sk.add_equiv; try refl. eapply Sk.add_comm; et. }
+    erewrite (Mod.get_modsem_Proper md_src0); try eapply T.
+    2: { eapply Sk.wf_mon; et. rewrite sim_sk0. rewrite sim_sk1. rewrite EXT. refl. }
+    assert(U: sk_tgt ⊕ (Mod.sk md_tgt0 ⊕ Mod.sk md_tgt1) ≡ (sk_tgt ⊕ Mod.sk md_tgt1) ⊕ Mod.sk md_tgt0).
+    { rewrite <- ! Sk.add_assoc. eapply Sk.add_equiv; try refl. eapply Sk.add_comm; et. }
+    erewrite (Mod.get_modsem_Proper md_tgt0); try eapply U.
+    2: { ss. }
+    eapply sim_modsem0; ss.
+    2: { rewrite <- U; et. }
+    rewrite EXT. rewrite sim_sk1. refl.
+  - assert(T: sk_src ⊕ (Mod.sk md_src0 ⊕ Mod.sk md_src1) ≡ (sk_src ⊕ Mod.sk md_src0) ⊕ Mod.sk md_src1).
+    { rewrite <- ! Sk.add_assoc. eapply Sk.add_equiv; try refl. }
+    erewrite (Mod.get_modsem_Proper md_src1); try eapply T.
+    2: { eapply Sk.wf_mon; et. rewrite sim_sk0. rewrite sim_sk1. rewrite EXT. refl. }
+    assert(U: sk_tgt ⊕ (Mod.sk md_tgt0 ⊕ Mod.sk md_tgt1) ≡ (sk_tgt ⊕ Mod.sk md_tgt0) ⊕ Mod.sk md_tgt1).
+    { rewrite <- ! Sk.add_assoc. eapply Sk.add_equiv; try refl. }
+    erewrite (Mod.get_modsem_Proper md_tgt1); try eapply U.
+    2: { ss. }
+    eapply sim_modsem1; ss.
+    2: { rewrite <- U; et. }
+    rewrite EXT. rewrite sim_sk0. refl.
 Qed.
 
 Theorem adequacy
@@ -1406,28 +1422,32 @@ Theorem adequacy
 .
 Proof.
   ii. unfold Mod.compile, Mod.enclose in *.
-  destruct (classic (Mod.wf (ctx ⊕ md_src))).
-  2:{ eapply ModSem.compile_not_wf. ss. }
+  destruct (classic (Mod.wf (ctx ⊕ md_tgt))).
+  2:{ eapply ModSem.compile_not_wf in PR; ss. subst. eapply Beh.nb_bottom. }
   pose (sk_tgt := (Mod.sk (ctx ⊕ md_tgt))).
   pose (sk_src := (Mod.sk (ctx ⊕ md_src))).
-  destruct (classic (Sk.wf (Mod.sk md_src))); rename H0 into SKWF.
-  2: { eapply ModSem.initial_itr_not_wf. intro T. eapply SKWF. inv T; ss. eapply Sk.wf_mon; et. r. esplits; et.
+  destruct (classic (Sk.wf (Mod.sk md_tgt))); rename H0 into SKWF.
+  2: { eapply ModSem.initial_itr_not_wf in PR; ss.
+       { subst. eapply Beh.nb_bottom. }
+       intro T. eapply SKWF. inv T; ss. eapply Sk.wf_mon; et. r. esplits; et.
        rewrite Sk.add_comm; et. refl. }
-  assert (SKEQ: sk_tgt ≡ sk_src).
-  { unfold sk_src, sk_tgt. ss. inv SIM. spc sim_sk0. rewrite sim_sk0. refl. }
+  (* assert (SKEQ: sk_tgt ≡ sk_src). *)
+  (* { unfold sk_src, sk_tgt. ss. inv SIM. spc sim_sk0. rewrite sim_sk0. refl. } *)
+  assert(EXT: Sk.extends sk_src sk_tgt).
+  { subst sk_src sk_tgt. ss. inv SIM. rewrite sim_sk0. refl. }
 
   rr in H. unfold Mod.enclose in *. fold sk_src in H. des. inv WF.
   {
     folder.
     inv SIM. ss.
     exploit sim_modsem0.
-    { instantiate (1:=sk_src).
-      subst sk_src. r. esplits; et. rewrite Sk.add_comm. rewrite sim_sk0; ss. refl. }
+    { refl. }
     { eauto. }
-    intro T.
+    intro T; des.
     eapply ModSemPair.adequacy; revgoals; et.
     2: {
-      eapply ModSemPair.compose; erewrite <- Mod.get_modsem_Proper; et; try by (eapply Sk.wf_equiv; [sym; et|]; ss).
+      eapply ModSemPair.compose.
+      - erewrite <- Mod.get_modsem_Proper; et; try by (eapply Sk.wf_equiv; [sym; et|]; ss).
       - eapply ModSemPair.self_sim.
       - eapply sim_modsem0; et.
         { r. subst sk_tgt. esplits. rewrite Sk.add_comm; refl. }
